read(mil): finish §6.3

MIL/C06_Discrete_Mathematics/S03_Inductive_Structures.lean
@@ -61,12 +61,19 @@ theorem map_map' (f : α → β) (g : β → γ) (as : List α) :
   . rfl
   . simp [map, ih]
 
-def reverse : List α → List α := sorry
+def reverse : List α → List α -- use the TCO version here and you're buried
+  | [] => []
+  | a :: as => reverse as ++ [a]
 
 theorem reverse_append (as bs : List α) : reverse (as ++ bs) = reverse bs ++ reverse as := by
-  sorry
+  induction' as with a as ih
+  . simp [reverse]
+  . simp [reverse, ih, append_assoc]
 
-theorem reverse_reverse (as : List α) : reverse (reverse as) = as := by sorry
+theorem reverse_reverse (as : List α) : reverse (reverse as) = as := by
+  induction' as with a as ih
+  . simp [reverse]
+  . simp [reverse, reverse_append, ih]
 
 end MyListSpace3
 
@@ -97,14 +104,27 @@ theorem size_le : ∀ t : BinTree, size t ≤ 2^depth t - 1
           have : 0 < 2 ^ max l.depth r.depth := by simp
           omega
 
-theorem depth_le_size : ∀ t : BinTree, depth t ≤ size t := by sorry
+theorem depth_le_size : ∀ t : BinTree, depth t ≤ size t
+  | empty    => by simp [depth, size]
+  | node l r => by
+    simp only [depth, size]
+    calc max (depth l) (depth r) + 1
+      ≤ max (size l) (size r) + 1 := by
+          gcongr <;> apply depth_le_size
+    _ ≤ size l + size r + 1 := by field_simp
 
-def flip : BinTree → BinTree := sorry
+def flip : BinTree → BinTree
+  | empty    => empty
+  | node l r => node (flip r) (flip l)
 
 example: flip  (node (node empty (node empty empty)) (node empty empty)) =
-    node (node empty empty) (node (node empty empty) empty) := sorry
+    node (node empty empty) (node (node empty empty) empty) := by rfl
 
-theorem size_flip : ∀ t, size (flip t) = size t := by sorry
+set_option pp.fieldNotation false in
+theorem size_flip : ∀ t, size (flip t) = size t := by
+  intro t; induction t with
+  | empty => rfl
+  | node l r ih1 ih2 => simp [flip, ih1, ih2, size]; group
 end BinTree
 
 inductive PropForm : Type where
@@ -152,9 +172,16 @@ def subst : PropForm → ℕ → PropForm → PropForm
   | impl A B, m, C => impl (A.subst m C) (B.subst m C)
 
 theorem subst_eq_of_not_mem_vars :
-    ∀ (A : PropForm) (n : ℕ) (C : PropForm), n ∉ A.vars → A.subst n C = A := sorry
+    ∀ (A : PropForm) (n : ℕ) (C : PropForm), n ∉ A.vars → A.subst n C = A := by
+  intros A n C nivar
+  induction A <;> simp [vars, subst, *] at *
+  case var m => intros; simp_all
+  case conj | disj | impl => simp [*] at *
 
 theorem subst_eval_eq : ∀ (A : PropForm) (n : ℕ) (C : PropForm) (v : ℕ → Bool),
-  (A.subst n C).eval v = A.eval (fun m => if m = n then C.eval v else v m) := sorry
+  (A.subst n C).eval v = A.eval (fun m => if m = n then C.eval v else v m) := by
+  intros A n C v
+  induction A <;> simp [eval, subst, *] at *
+  case var m => by_cases (m = n) <;> simp [*, eval]
 
 end PropForm
